txn-data-consistency/EP+_TCCv_Invariants.thy
@@ -187,6 +187,10 @@ definition FTid_notin_rs where
 definition FTid_not_wr where
   "FTid_not_wr s cl \<longleftrightarrow> (\<forall>n k. n > cl_sn (cls s cl) \<longrightarrow> Tn (Tn_cl n cl) \<notin> wtxns_dom (svr_state (svrs s k)))"
 
+definition Fresh_wr_notin_Wts_dom where
+  "Fresh_wr_notin_Wts_dom s cl \<longleftrightarrow> (\<forall>cclk keys kv_map k. cl_state (cls s cl) \<in> {Idle, RtxnInProg cclk keys kv_map} \<longrightarrow>
+    Tn (get_txn s cl) \<notin> wtxns_dom (svr_state (svrs s k)))"
+
 definition Fresh_wr_notin_rs where
   "Fresh_wr_notin_rs s cl \<longleftrightarrow> (\<forall>k t cts kv_map cclk keys cts' sts' lst' v' rs'.
     svr_state (svrs s k) t = Commit cts' sts' lst' v' rs' \<and>
@@ -195,9 +199,10 @@ definition Fresh_wr_notin_rs where
      cl_state (cls s cl) \<in> {Idle, WtxnPrep kv_map, WtxnCommit cts kv_map})
      \<longrightarrow> rs' (get_txn s cl) = None)" (* RtxnInProg case not proven *)
 
-definition Fresh_wr_notin_Wts_dom where
-  "Fresh_wr_notin_Wts_dom s cl \<longleftrightarrow> (\<forall>cclk keys kv_map k. cl_state (cls s cl) \<in> {Idle, RtxnInProg cclk keys kv_map} \<longrightarrow>
-    Tn (get_txn s cl) \<notin> wtxns_dom (svr_state (svrs s k)))"
+definition Once_in_rs where
+  "Once_in_rs s k t \<longleftrightarrow> (\<forall>t_wr cts ts lst v rs m t_wr' cts' ts' lst' v' rs'.
+    svr_state (svrs s k) t_wr = Commit cts ts lst v rs \<and> rs t = Some m \<and>
+    t_wr' \<noteq> t_wr \<and> svr_state (svrs s k) t_wr' = Commit cts' ts' lst' v' rs' \<longrightarrow> rs' t = None)"
 
 
 subsection \<open>monotonic lemmas and inequality of timestamps invariants\<close>
@@ -208,8 +213,8 @@ lemma svr_clock_monotonic:
 lemma cl_clock_monotonic:
   "state_trans s e s' \<Longrightarrow> cl_clock (cls s' cl) \<ge> cl_clock (cls s cl)" oops
 
-definition Pend_Wt_UB where
-  "Pend_Wt_UB s svr \<longleftrightarrow> (\<forall>ts \<in> pending_wtxns_ts (svr_state (svrs s svr)). ts \<le> svr_clock (svrs s svr))"
+definition Pend_le_Clk where
+  "Pend_le_Clk s svr \<longleftrightarrow> (\<forall>ts \<in> pending_wtxns_ts (svr_state (svrs s svr)). ts \<le> svr_clock (svrs s svr))"
 
 definition Prep_le_Clk where
   "Prep_le_Clk s svr \<longleftrightarrow>
@@ -219,11 +224,11 @@ definition Pend_lt_Prep where
   "Pend_lt_Prep s svr \<longleftrightarrow>
     (\<forall>t pd ts v. svr_state (svrs s svr) t = Prep pd ts v \<longrightarrow> pd < ts)"
 
-definition Clk_le_Lst where
-  "Clk_le_Lst s k \<longleftrightarrow> svr_lst (svrs s k) \<le> svr_clock (svrs s k)"
+definition Lst_le_Clk where
+  "Lst_le_Clk s k \<longleftrightarrow> svr_lst (svrs s k) \<le> svr_clock (svrs s k)"
 
-definition Pend_Wt_LB where
-  "Pend_Wt_LB s svr \<longleftrightarrow> (\<forall>ts \<in> pending_wtxns_ts (svr_state (svrs s svr)). svr_lst (svrs s svr) \<le> ts)"
+definition Lst_le_Pend where
+  "Lst_le_Pend s svr \<longleftrightarrow> (\<forall>ts \<in> pending_wtxns_ts (svr_state (svrs s svr)). svr_lst (svrs s svr) \<le> ts)"
 
 lemma min_pending_wtxns_monotonic:
   assumes "state_trans s e s'"
@@ -250,13 +255,25 @@ definition Get_lst_le_Lst where
 definition Lst_map_le_Lst where
   "Lst_map_le_Lst s cl k \<longleftrightarrow> (lst_map (cls s cl) k \<le> svr_lst (svrs s k))"
 
-definition Rlst_ge_Lst_map where
-  "Rlst_ge_Lst_map s cl k \<longleftrightarrow> (\<forall>t cts ts lst v rs rlst rts.
-    svr_state (svrs s k) t = Commit cts ts lst v rs \<and> rs (get_txn s cl) = Some (rts, rlst)
-      \<longrightarrow> lst_map (cls s cl) k \<le> rlst)" (* not proven *)
+definition Gst_le_Pend_t where
+  "Gst_le_Pend_t s cl \<longleftrightarrow> (\<forall>k pend_t prep_t v. 
+      svr_state (svrs s k) (get_wtxn s cl) = Prep pend_t prep_t v \<longrightarrow> gst (cls s cl) \<le> prep_t)"
 
-definition Get_lst_ge_Lst_map where
-  "Get_lst_ge_Lst_map s cl k \<longleftrightarrow> (\<forall>cts ts lst v rs.
+definition Gst_lt_Cts where
+  "Gst_lt_Cts s cl \<longleftrightarrow> (\<forall>k cts sts lst v rs. 
+      svr_state (svrs s k) (get_wtxn s cl) = Commit cts sts lst v rs \<longrightarrow> gst (cls s cl) < cts)" (*RInvoke & CommitW*)
+
+definition Gst_lt_Cl_Cts where
+  "Gst_lt_Cl_Cts s cl \<longleftrightarrow> (\<forall>cl' cts kv_map. cl_state (cls s cl') = WtxnCommit cts kv_map
+    \<longrightarrow> gst (cls s cl) < cts)" (*RInvoke & CommitW*)
+
+definition Lst_map_le_Rlst where
+  "Lst_map_le_Rlst s cl k \<longleftrightarrow> (\<forall>t cts ts lst v rs rlst rts.
+    svr_state (svrs s k) t = Commit cts ts lst v rs \<and> rs (get_txn s cl) = Some (rts, rlst)
+      \<longrightarrow> lst_map (cls s cl) k \<le> rlst)"
+
+definition Lst_map_le_Get_lst where
+  "Lst_map_le_Get_lst s cl k \<longleftrightarrow> (\<forall>cts ts lst v rs.
     svr_state (svrs s k) (get_wtxn s cl) = Commit cts ts lst v rs \<longrightarrow> lst_map (cls s cl) k \<le> lst)" (* not proven *)
 
 lemma lst_map_monotonic:
@@ -280,27 +297,8 @@ lemma gst_monotonic:
 definition Gst_le_Lst_map where
   "Gst_le_Lst_map s cl k \<longleftrightarrow> (gst (cls s cl) \<le> lst_map (cls s cl) k)"
 
-definition Pending_Wtxns_Inv where
-  "Pending_Wtxns_Inv s k \<longleftrightarrow> (\<forall>pend_t. pend_t \<in> pending_wtxns_ts (svr_state (svrs s k))
-    \<longleftrightarrow> (\<exists>t prep_t v. svr_state (svrs s k) t = Prep pend_t prep_t v))"
-
-definition Lst_Lt_Pdts where
-  "Lst_Lt_Pdts s k \<longleftrightarrow> (\<forall>t pend_t prep_t v. svr_state (svrs s k) t = Prep pend_t prep_t v \<longrightarrow> svr_lst (svrs s k) \<le> prep_t)"
-
 definition Rtxn_rts_le_Gst where
   "Rtxn_rts_le_Gst s cl \<longleftrightarrow> (\<forall>n ts. rtxn_rts s (Tn_cl n cl) = Some ts \<longrightarrow> ts \<le> gst (cls s cl))"
-
-definition Gst_le_Pend_t where
-  "Gst_le_Pend_t s cl \<longleftrightarrow> (\<forall>k pend_t prep_t v. 
-      svr_state (svrs s k) (get_wtxn s cl) = Prep pend_t prep_t v \<longrightarrow> gst (cls s cl) \<le> prep_t)"
-
-definition Gst_Lt_Cts where
-  "Gst_Lt_Cts s cl \<longleftrightarrow> (\<forall>k cts sts lst v rs. 
-      svr_state (svrs s k) (get_wtxn s cl) = Commit cts sts lst v rs \<longrightarrow> gst (cls s cl) < cts)" (*RInvoke & CommitW*)
-
-definition Gst_Lt_Cl_Cts where
-  "Gst_Lt_Cl_Cts s cl \<longleftrightarrow> (\<forall>cl' cts kv_map. cl_state (cls s cl') = WtxnCommit cts kv_map
-    \<longrightarrow> gst (cls s cl) < cts)" (*RInvoke & CommitW*)
 
 
 subsection \<open>Commit Order Invariants\<close>
